\documentclass[12pt]{article}%
\usepackage{amsfonts}
\usepackage{fancyhdr}
\usepackage{comment}
\usepackage[a4paper, top=2.5cm, bottom=2.5cm, left=2.2cm, right=2.2cm]%
{geometry}
\usepackage{times}
\usepackage{amsmath}
\usepackage{changepage}
\usepackage{amssymb}
\usepackage{graphicx}%
\setcounter{MaxMatrixCols}{30}
\newtheorem{theorem}{Theorem}
\newtheorem{acknowledgement}[theorem]{Acknowledgement}
\newtheorem{algorithm}[theorem]{Algorithm}
\newtheorem{axiom}{Axiom}
\newtheorem{case}[theorem]{Case}
\newtheorem{claim}[theorem]{Claim}
\newtheorem{conclusion}[theorem]{Conclusion}
\newtheorem{condition}[theorem]{Condition}
\newtheorem{conjecture}[theorem]{Conjecture}
\newtheorem{corollary}[theorem]{Corollary}
\newtheorem{criterion}[theorem]{Criterion}
\newtheorem{definition}[theorem]{Definition}
\newtheorem{example}[theorem]{Example}
\newtheorem{exercise}[theorem]{Exercise}
\newtheorem{lemma}[theorem]{Lemma}
\newtheorem{notation}[theorem]{Notation}
\newtheorem{problem}[theorem]{Problem}
\newtheorem{proposition}[theorem]{Proposition}
\newtheorem{remark}[theorem]{Remark}
\newtheorem{solution}[theorem]{Solution}
\newtheorem{summary}[theorem]{Summary}
\newenvironment{proof}[1][Proof]{\textbf{#1.} }{\ \rule{0.5em}{0.5em}}

\newcommand{\Q}{\mathbb{Q}}
\newcommand{\R}{\mathbb{R}}
\newcommand{\C}{\mathbb{C}}
\newcommand{\Z}{\mathbb{Z}}

\newcommand{\E}{\mathrm{E}}
\newcommand{\Var}{\mathrm{Var}}
\newcommand{\Cov}{\mathrm{Cov}}

\begin{document}

\title{Math 545 - PDEs - Homework 3}
\author{YingLi Li, Fernando Herrera Valverde, Laurette Hamlin}
\date{\today}
\maketitle

\begin{enumerate}
    \item 2.4.1 \\
    Solution: 

  \[ 
    \begin{aligned}
        u(x, t) & =\frac{1}{\sqrt{4 \pi k t}} \int_{-\infty}^{+\infty} e^\frac{-(x-y)^{2}}{4kt}\phi(y) d y\\
        & =\frac{1}{\sqrt{4 \pi kt}} \int_{-l}^{l} e^\frac{-(x-y)^{2}}{4kt}  d y\\
        & =\frac{1}{\sqrt{\pi}} \int_{(-l-x) / \sqrt{4 k t}}^{(l-x) / \sqrt{4 k t}} e^{-p^{2}} d p \\
        & =\frac{1}{2}\left\{ E r f\left[\frac{x+l}{\sqrt{4 k t}}\right]-E r f\left[\frac{x-l}{\sqrt{4 k t}}\right]\right\} .
        \end{aligned} 
\]

    \item 2.4.15 \\
    Solution: Assume there exists two another solution $v(x,t)$ also satisfies the diffusion problem.

    Let $w(x,t)=u(x,t)-v(x,t)$, since the problem is linear, we obtain 
    \begin{equation*}
        \begin{cases}
            w_{t}-kw_{xx}=0,
            \\
            w(x,0)=0,
            \\
            w_{x}(0,t)=0,\quad w_{x}(l,t)=0.
        \end{cases} 
    \end{equation*}
 From the energy method, 
 \[\frac{d}{d t} \int_{0}^{l} \frac{1}{2} w^{2}(x, t) d x=-k \int_{0}^{l} w_{x}^{2}(x, t) d x \leq 0\]
 The initial condition is $w(x,0)=0$, thus $ \int_{0}^{l} \frac{1}{2} w^{2}(x, t) d x \leq  \int_{0}^{l} \frac{1}{2} w^{2}(x, 0) dx =0.$
 
 Therefore, $u(x,t)-v(x,t)=w(x,t)=0 \implies u(x,t)=v(x,t),$ the solution of the diffusion problem is unique.

 \item 2.4.16 \\
 Solution: Let $v(x,t)=e^{-bt}u(x,t)$, plug $v(x,t)$ to the equation:
 \begin{equation*}
    \begin{cases}
        v_{t}-kv_{xx}=0,
        \\
        v(x,0)=\phi(x).
    \end{cases} 
 \end{equation*}
 The solution is $v(x, t) =\frac{1}{\sqrt{4 \pi k t}} \int_{-\infty}^{+\infty} e^\frac{-(x-y)^{2}}{4kt}\phi(y) dy$.

 Thus, $u(x,t)=e^{-bt}u(x,t)=\frac{e^{-bt}}{\sqrt{4 \pi k t}} \int_{-\infty}^{+\infty} e^\frac{-(x-y)^{2}}{4kt}\phi(y) dy$.

\item 2.4.18\\
Solution: Let $v(x-Vt,t)=u(x,t)$,i.e. $v(x,t)=u(x+Vt,t)$ plug into the equation,
\begin{equation*}
    \begin{cases}
        u_{t}-ku_{xx}+Vu_{x}=v_{t}-kv_{xx}=0,
        \\
        v(x,0)=u(x, 0)=\phi(y).
    \end{cases} 
\end{equation*}
The solution is $v(x, t) =\frac{1}{\sqrt{4 \pi k t}} \int_{-\infty}^{+\infty} e^\frac{-(x-y)^{2}}{4kt}\phi(y) dy$.

Thus, $u(x,t)=v(x-Vt, t)=\frac{1}{\sqrt{4 \pi k t}} \int_{-\infty}^{+\infty} e^\frac{-(x-Vt-y)^{2}}{4kt}\phi(y) dy$.


\item 4.1.3\\
Solution: The equation is 
\begin{equation*}
    \begin{cases}
        u_{t}=iu_{xx}, x\in (0,l),
        \\
        u(0,t)=u(l,t)=0.
    \end{cases}
\end{equation*}
Assumen $u(x,t)=X(x)T(t)$, pulg into the equation, we obtain 
\begin{equation}\label{T}
        \frac{1}{i}\frac{T'(t)}{T(t)}=-\lambda,
\end{equation}
\begin{equation}\label{X}
    \frac{X''(t)}{X(t)}=-\lambda.
\end{equation}
Where $\lambda =\mu^2$.

Solve equation (\ref*{T}), $T_{n}(t)=Ce^{i\lambda_{n} T}$.

Solve equation (\ref*{X}), $X_{n}(x)=A_{n}cos\mu_{n}x+B_{n}sin\mu_{n}x, n\in \mathbb{Z}, $ from the initial condition,
\begin{equation*}
    \begin{cases}
    X_{n}(0)=A_{n}=0,
    \\
    X_{n}(l)=B_{n}sin\mu_{n}l=0 \implies \mu_{n} = \frac{n\pi}{l}. n\in \mathbb{Z}.
\end{cases}
\end{equation*}
Thus, $X_{n}(t)=B_{n}sin\frac{n\pi}{l}x, n\in \mathbb{Z}$.

And $u(x,t)=X(x)T(t)=\sum_{n=0}^{\infty  } X_{n}(x)T_{n}(t) \sum_{n=0}^{\infty  } \widetilde{B_{n}}  e^{i(\frac{n\pi}{l})^2T}sin\frac{n\pi}{l}x, n\in \mathbb{Z}$, where $\widetilde{B_{n}}=B_{n}C_{n}$.




\end{enumerate}
   
    
    

\end{document}
