% TODO: check spelling!!!
\documentclass{article}
\usepackage{enumitem} % Change enumerate
\setlist[enumerate,2]{label=(\alph*)} % Change enumerate
\usepackage{amsmath}
\title{MATH 545: Homework 1}
\author{Yingli, Laurette, Fernando}
\date{September 9th, 2023}
\begin{document}
\maketitle
\begin{enumerate}
\item Solve the following ODEs.
\begin{enumerate}
	\item $(y')^2 -4y +4 = 0$

		Solution:

		We proceed by separation of variables.

		\begin{align*}
			(y')^2 -4y +4 = 0 \\
			\iff (y')^2 = 4y -4
		\end{align*}
		This means that we have two options for $y'$, namely:
		\[y' = \pm 2\sqrt{y-1}.\]
		Then:
		\begin{align*}
			y' = \pm 2\sqrt{y-1} \\
			\iff \frac{dy}{dx} = \pm 2\sqrt{y-1} \\
			\iff \frac{dy}{\pm 2\sqrt{y-1}} = dx
		\end{align*}
		Integrating we get:
		$\pm \sqrt{y-1} = x+c$,

		then
		\begin{equation} \label{sol}
			y = (x+c)^2 + 1.
		\end{equation}
		Now we test the function we found. First we notice that
		\begin{equation} \label{sol_deriv}
			y' = 2(x+c),
		\end{equation}
		then we substitute (\ref{sol}) and (\ref{sol_deriv}) in the original equation to obtain
		\begin{align*}
			(2(x+c))^2 -4((x+c)^2 + 1) +4 =0 \\
			\iff 4(x+c)^2 -4(x+c)^2 -4 + 4 =0,
		\end{align*}
		so the function we found is in fact a solution.

	\item $(y\;\text{sin} x + xy\;\text{cos}x)dx + (x\;\text{sin}x + 1)dy = 0$

		Solution:
		
		We start by showing that this equation is exact.

		In this case we have $M(x,y) = y\text{sin}x + xy\text{cos}x$ and $N(x,y) = x\text{sin}x + 1$.

		Then $\frac{\partial M(x,y)}{\partial y} = \text{sin}x + x\text{cos}x$ and $\frac{\partial N(x,y)}{\partial x} = \text{sin}x + x\text{cos}x$

		i.e. $\frac{\partial M(x,y)}{\partial y} = \frac{\partial N(x,y)}{\partial x}$.

		Hence, the equation is exact.

		Now we solve $\frac{\partial f(x,y)}{\partial y} = x\text{sin}x + 1$. Integrating with respect to $y$ we get
		\[f(x,y) = y(x\text{sin}x +1) + h(x)\]
		In order to determine $h(x)$ we differentiate with
		respect to $x$ to obtain
		\[\frac{\partial f(x,y)}{\partial x} = y(\text{sin}x+x\text{cos}x) + h'(x).\]
		This must equal $M(x,y)$, so:
		\[y(\text{sin}x+x\text{cos}x) + h'(x) = y\text{sin}x + xy\text{cos}x,\]
		this implies that $h'(x)=0$, which means that $h(x) = c_1$.
		So the solution is implicitely given by:
		\begin{align*}
			f(x,y) = y(x\text{sin}x +1) + c_1 = c_2 \\
			\iff y(x\text{sin}x +1) = c \\
		\end{align*}
		In order to verify that this function solves the equation we calculate the differential.

		\[\frac{\partial f}{\partial x} = y\text{sin}x + xy\text{cos}x\]
		\[\frac{\partial f}{\partial y} = x\text{sin}x + 1\]
		So when we calculate $df$ we get:
		\[ df = (y\text{sin}x + xy\text{cos}x)dx + (x\text{sin}x + 1)dy =0\]
		Hence, this solves the equation.
		
	\item $y' + (2/x)y = x$; initial condition $y(1)=0$

		Solution:

		We begin by solving the homogeneous equation

		\[ \frac{dy}{dx} + \frac{2y}{x} = 0\]

		by separation of variables

		\[\frac{dy}{y} = -2\frac{dx}{x} \implies ln(y) = -2ln(x) + c_1 \implies y = \frac{c_2}{x^2}.\]

		% TODO: FIX THIS!!!!
		% This can be simplified !!
		Now we solve the equation:

		\begin{equation} \label{sol_homo}
			y(x) = q(x)u(x)
		\end{equation}

		where $q(x) = \frac{1}{x^2}$. For this we substitute (\ref{sol_homo}) into the original equation.
		\begin{align}
			y' + (2/x)y = x \nonumber \\
			\iff q'(x)u(x) +q(x)u'(x) + (2/x)q(x)u(x) = x \nonumber \\
			\iff \frac{-2}{x^3}	u(x) +\frac{1}{x^2}u'(x) + (2/x)\frac{1}{x^2}u(x) = x \nonumber \\
			\iff \frac{1}{x^2}u'(x) = x \nonumber \\
			\iff u'(x) = x^3 \nonumber \\
			\implies u(x) = \frac{x^4}{4} + c \label{ux}.
		\end{align}

		Since we know $q(x)$ we can sustitute (\ref{ux}) into (\ref{sol_homo}) to get:
		\[y(x) = \frac{1}{x^2}\left(\frac{x^4}{4}+c\right) = \frac{x^2}{4} + \frac{c}{x^2}.\]

		The initial condition is $y(1)=0$ so $y(1)=\frac{1}{4} + c= 0 \implies c=-\frac{1}{4}$,
		then
		\[y(x) = \frac{1}{x^2}\left(\frac{x^4}{4}+c\right) = \frac{x^2}{4} - \frac{1}{4x^2}.\]

		Now we check that the function found is a solution.

		First, the initial condition:
		\[y(1)= \frac{1^2}{4} - \frac{1}{4\cdot 1^2} =0.\]

		Secondly, we check that it satisfies the equation.
		\[y'+(2/x)y = \left(\frac{x}{2} + \frac{1}{2x^3}\right) +(2/x)\left(\frac{x^2}{4} - \frac{1}{4x^2}\right) = x.\]
		Hence the function solves the equation.


\end{enumerate}
\item Strauss section 1.2
	\begin{enumerate}
		\item Exercise 1. Solve the first-order equation
			$2u_t +3u_ x =0$ with the auxiliary condition $u=\text{sin}x$ when $t=0.$

			Solution:

			We solved this type of equation in class.
			the solution is 

			$u(t,x)=f(2x-3t)$

			Where $f$ is any sufficiently nice function.

			Using the initial condition we get:
			\[u(0,x)=f(2x)=\text{sin}x,\]
			so $f(x)=\text{sin}\left(\frac{x}{2}\right)$.
			Finally we have:
			\[u(t,x)=\text{sin}\left(x-\frac{3}{2}t\right)\]
			We check by differentiating.

			\[u_x=\text{cos}\left(x-\frac{3}{2}t\right)\]
			\[u_t=-\frac{3}{2}\text{cos}\left(x-\frac{3}{2}t\right)\]

			so
			\[ 2u_t +3u_x=-3\text{cos}\left(x-\frac{3}{2}t\right) + 3\text{cos}\left(x-\frac{3}{2}t\right)=0\]

			As for the initial condition:
			\[u(0,x)=\text{sin}\left(x-\frac{3}{2}\cdot0\right)=\text{sin}x.\]

			Hence $u(t,x)$ is in fact a solution to the PDE.

		\item Exercise 2. Solve the equation $3u_y + u_{xy} =0$

			Solution:
			% TODO: Maybe we should frame this in terms of antiderivaties!!!

			Let $v=u_y$, then the equation becomes:
			% TODO this align looks ugly, make it nicer if time allows
			\begin{align*}
				 3v+v_x=0 \\
				 \iff 3v+\frac{\partial v}{\partial x}=0 \\
				 \iff \frac{\partial v}{\partial x}=-3v \\
				 \iff \frac{\partial v}{v}=-3\partial x \\
				 \iff ln(v) = -3x + f(y) \\
				 \iff v = g(y)e^{-3x}
			\end{align*}
			Since $v=u_y$ we have:
			\[u(x,y)=\int vdy = e^{-3x}\int g(y)dy + f(x).\]

		\item Exercise 6. Solve the equation $\sqrt{1-x^2}u_x+u_y=0$ with the condition $u(0, y)=y.$
		
            Solution: The charecteristic curve satisfies the ODE: 
            \[ \frac{dy}{dx}=\frac{1}{\sqrt{1-x^2}}\]
			To solve the solution, we separate variables: 		
			\[ dy=\frac{1}{\sqrt{1-x^2}}dx.\]
			By intergral, \[y= arcsinx + c .\]
			Since $u(x,y)$ is a constant on each such curve, so
			\[ u(x,y)=f(c)=f(y - arcsinx).\]
			Since the initial condition is $u(0,y)=y$, then $u(0,y)=f(y)=y.$

			Finally we have:
			\[u(t,x)=y - arcsinx.\]
			We check our solution by differentiating:
			\[u_x=-\frac{1}{\sqrt{1-x^2}}\]
			\[u_y=1\]
			so \[\sqrt{1-x^2}u_x+u_y=-\sqrt{1-x^2} \cdot \frac{1}{\sqrt{1-x^2}}+1=0.\]

			Hence $u(t,x)$ is in fact a solution to the PDE.


		\item Exercise 8. Solve $au_x+bu_y+cu=0.$
		Solution:
		By using coordinate method: let $x'=ax+by$, $y'=bx-ay$.

		% TODO: Change the variable to something else, like \tilda to avoid confusion with derivative
		Replace all $x$ and $y$ derivatives by $x'$ and $y'$ derivatives.

		By the chain rule, \[u_x=\frac{\partial u}{\partial x}=\frac{\partial u}{\partial x'}\cdot{\partial x'}{\partial x}+\frac{\partial u}{\partial y'}\cdot{\partial y'}{\partial x}=au_{x'}+bu_{y'},\]
		\[u_y=\frac{\partial u}{\partial y}=\frac{\partial u}{\partial x'}\cdot{\partial x'}{\partial y}+\frac{\partial u}{\partial y'}\cdot{\partial y'}{\partial y}=bu_{x'}-au_{y'}.\]

		Hence,
		% TODO: Improve this!!!
		\begin{align*}
			au_x+bu_y+cu=\\
			a\left(au_{x'}+bu_{y'} \right)+b\left(bu_{x'}-au_{y'}\right)=\left(a^2+b^2\right)u_{x'}+cu=0.
		\end{align*}
		We seperate variables, \[\frac{\partial u}{u}=-\frac{c}{a^2+b^2}\partial x'.\]
		Hence, \[\ln u = -\frac{c}{a^2+b^2}x' +g(y'),\] so that \[ u = f(y')e^{-\frac{c}{a^2+b^2}x'}.\]
		Thus the solution is  \[ u = f(bx-ay)e^{-\frac{c}{a^2+b^2}(ax+by)}.\]

		We check our solution by differentiating:
		\[u_x= b f'(bx-ay)e^{-\frac{c}{a^2+b^2}(ax+by)} -\frac{ac}{a^2+b^2} \cdot e^{-\frac{c}{a^2+b^2}(ax+by)}f(bx-ay),\]
		\[u_y= -a f'(bx-ay)e^{-\frac{c}{a^2+b^2}(ax+by)} -\frac{bc}{a^2+b^2} \cdot e^{-\frac{c}{a^2+b^2}(ax+by)}f(bx-ay),\]
		% TODO: Improve this!!
		So
		% TODO: ask Yingli if we should keep the e^f instead of just f
		\begin{align*}
			au_x+bu_y+cu= \\
			a\cdot b f'(bx-ay)e^{-\frac{c}{a^2+b^2}(ax+by)} \\
			-\frac{ac}{a^2+b^2} \cdot e^{-\frac{c}{a^2+b^2}(ax+by)}f(bx-ay) \\
			-b a f'(bx-ay)e^{-\frac{c}{a^2+b^2}(ax+by)} \\
			-\frac{bc}{a^2+b^2} \cdot e^{-\frac{c}{a^2+b^2}(ax+by)}f(bx-ay) \\
			= 0
		\end{align*}
	\end{enumerate}
\item Strauss section 1.3
	\begin{enumerate}
		\item Exercise 4. Suppose that some particles which are
			suspended in a liquid medium would be pulled down
			at a constant velocity $V > 0$ by gravity in the
			absence of diffusion. Taking account of the
			diffusion, find the equation for the concentration
			of particles. Assume homogeneity in the horizontal
			directions $x$ and $y$. Let the $z$ axis point
			upwards.

			Solution:

			% TODO: Add a drawing if time allows

			Since we are assuming homogeneity in the horizontal
			directions, the concentration $u$ depends only on $z$.
			Let $u(z,t)$ be the concentration. We proceed as the
			book does for diffusion.

			The mass in the region of the fluid contained between
			$z_0$ and $z_1$ is given by:

			\begin{equation} \label{change_of_mass}
				M(t) = \int_{z_0}^{z_1} u(z,t)dz, \text{ so }
			\frac{dM}{dt}=\int_{z_0}^{z_1}u_t(z,t)dz.
			\end{equation}

			The mass in this section of the fluid cannot change
			except by flowing in or out if its ends.

			There are two proceses that regulate the entrance and
			exit of particles into this region of the fluid.
			The first one is difusion and the second one is the
			movement of the particles due to gravity acting on
			them.

			For diffusion we have:
			\[\frac{dM_{diffusion}}{dt}=ku_z(z_1,t)-ku_z(z_0,t),\]
			just like the example in the book.

			For the movement of particles due to gravity we have:
			\[\frac{dM_{gravity}}{dt} = Vu(z_1,t) - Vu(z_0,t).\]

			Now the total change in the mass per unit of time is
			the sum of this two componenets.
			\begin{align*}
				\frac{dM}{dt}&=\frac{dM_{diffusion}}{dt}+\frac{dM_{gravity}}{dt} \\
				\frac{dM}{dt}&=ku_z(z_1,t)-ku_z(z_0,t) + Vu(z_1,t) - Vu(z_0,t)
			\end{align*}
			Using equation (\ref{change_of_mass}) we get:
			\[\int_{z_0}^{z_1}u_t(z,t)dz= ku_z(z_1,t)-ku_z(z_0,t) + Vu(z_1,t) - Vu(z_0,t).\]
			Differentiating with respect to $z_1$ we get:
			\[
				u_t=ku_{zz}+Vu_z.
			\]

		\item Exercise 8. For the hydrigen atom, if $ \int \left | u^2 \right | d \vec{x } =1$, at $t=0$, show thath the same is true at all later times.
		
		Solution: If we want to show that $ \int \left | u^2 \right | d \vec{x } =1$ is true at all times, we should show that $\frac{d}{dt}\int \left | u^2 \right | d \vec{x } =0$.
                  
		Since
		\begin{align*}
			 \frac{d}{dt}\int \left | u^2 \right | d \vec{x } =&
			 \int \frac{d}{dt} \left | u^2 \right | d \vec{x }=
			 \int \frac{d}{dt} \left(uu^* \right)d \vec{x }=
			 \int\left(  u_{t}u^*+uu_{t}^*\right) d \vec{x }
		\end{align*}

		According to Schr$\ddot{o}$dinger equation: 
		\[-\mathrm{i}hu_{t}=\frac{h^2}{2m}\triangle u+ \frac{e^2}{r}u,\]
		we will obtain that
		\[u_{t}=\frac{\mathrm{i}h}{2m}\triangle u+ \frac{ie^2}{hr}u,\]
		\[u_{t}^*=-\frac{\mathrm{i}h}{2m}\triangle u^*-\frac{ie^2}{hr}u^*,\]

		Therefore,

			\[u_{t}u^*+uu_{t}^*=(\frac{\mathrm{i}h}{2m}\triangle u+\frac{ie^2}{hr}u)u^*-u(\frac{\mathrm{i}h}{2m}\triangle u^*+\frac{ie^2}{hr}u^*)= \frac{\mathrm{i}h}{2m} (u^*\triangle u -u\triangle u^*) \]
			Since, \[\nabla \cdot (\nabla u \cdot u^* -u\cdot \nabla u^*)= \triangle u \cdot u^*+ \nabla u\cdot \nabla u^*- \nabla u\cdot \nabla u^*- u\cdot\triangle u^*=\triangle u \cdot u^*-u\cdot\triangle u^*,\]
			Therefore, \[ \frac{d}{dt}\int \left | u^2 \right | d \vec{x }=\int(u_{t}u^*+uu_{t}^*)  d \vec{x } = \frac{\mathrm{i}h}{2m}\int(u^*\triangle u -u\triangle u^*)d \vec{x }=\frac{\mathrm{i}h}{2m}\int \nabla \cdot (\nabla u \cdot u^* -u\cdot \nabla u^*)d \vec{x }\]
            In $\mathrm{R}^3$ space, let $B(r)$ be a ball with origin center and radius r.
			Then \[ \frac{d}{dt}\int_{\mathrm{R^3} }^{}  \left | u^2 \right | d \vec{x }= \lim_{r \to \infty}\int_{B(r)}\frac{d}{dt} \left | u^2 \right | d \vec{x }= \frac{\mathrm{i}h}{2m}\lim_{r \to \infty}\iiint_{r}^{} \nabla \cdot (\nabla u \cdot u^* -u\cdot \nabla u^*)d \vec{x }.\]
			From divergence theorem,
			\[\iiint_{r}^{} \nabla \cdot (\nabla u \cdot u^* -u\cdot \nabla u^*)dx dy dz= \iint_{\partial B(r)}^{}(\nabla u \cdot u^* -u\cdot \nabla u^*) \cdot \bar{n} dS.	\]
			Assume that $u$ and $\nabla u \to 0$ fast enough as $\left | \vec{x} \right | \to 0$, then we get
		
		\[ \lim_{r \to \infty}\iiint_{r}^{} \nabla \cdot (\nabla u \cdot u^* -u\cdot \nabla u^*)d \vec{x } =0,\]

		Therefore, \[ \frac{d}{dt}\int \left | u^2 \right | d \vec{x }=\frac{\mathrm{i}h}{2m}\lim_{r \to \infty}\iiint_{r}^{} \nabla \cdot (\nabla u \cdot u^* -u\cdot \nabla u^*)d \vec{x }=0,\]
			which means that at all later times, $ \int \left | u^2 \right | d \vec{x } =1$.
		
	\end{enumerate}
\item Strauss section 1.4
	\begin{enumerate}
		\item Exercise 1.
		\item Exercise 2.
	\end{enumerate}
\item Strauss section 1.5
	\begin{enumerate}
		\item Exercise 1.
		\item Exercise 4.
	\end{enumerate}
\end{enumerate}

\end{document}
