\documentclass[12pt]{article}%
\usepackage{amsfonts}
\usepackage{fancyhdr}
\usepackage{comment}
\usepackage[a4paper, top=2.5cm, bottom=2.5cm, left=2.2cm, right=2.2cm]%
{geometry}
\usepackage{times}
\usepackage{amsmath}
\usepackage{changepage}
\usepackage{amssymb}
\usepackage{graphicx}%
\setcounter{MaxMatrixCols}{30}
\newtheorem{theorem}{Theorem}
\newtheorem{acknowledgement}[theorem]{Acknowledgement}
\newtheorem{algorithm}[theorem]{Algorithm}
\newtheorem{axiom}{Axiom}
\newtheorem{case}[theorem]{Case}
\newtheorem{claim}[theorem]{Claim}
\newtheorem{conclusion}[theorem]{Conclusion}
\newtheorem{condition}[theorem]{Condition}
\newtheorem{conjecture}[theorem]{Conjecture}
\newtheorem{corollary}[theorem]{Corollary}
\newtheorem{criterion}[theorem]{Criterion}
\newtheorem{definition}[theorem]{Definition}
\newtheorem{example}[theorem]{Example}
\newtheorem{exercise}[theorem]{Exercise}
\newtheorem{lemma}[theorem]{Lemma}
\newtheorem{notation}[theorem]{Notation}
\newtheorem{problem}[theorem]{Problem}
\newtheorem{proposition}[theorem]{Proposition}
\newtheorem{remark}[theorem]{Remark}
\newtheorem{solution}[theorem]{Solution}
\newtheorem{summary}[theorem]{Summary}
\newenvironment{proof}[1][Proof]{\textbf{#1.} }{\ \rule{0.5em}{0.5em}}

\newcommand{\Q}{\mathbb{Q}}
\newcommand{\R}{\mathbb{R}}
\newcommand{\C}{\mathbb{C}}
\newcommand{\Z}{\mathbb{Z}}

\newcommand{\E}{\mathrm{E}}
\newcommand{\Var}{\mathrm{Var}}
\newcommand{\Cov}{\mathrm{Cov}}

\begin{document}

\title{Math 545 - PDEs - Homework 2}
\author{YingLi Li, Fernando Herrera Valverde, Laurette Hamlin}
\date{\today}
\maketitle

\begin{enumerate}
    \item Strauss Section 1.5 \smallskip
    \begin{enumerate}
        \item Exercise 2 \smallskip \\
        Consider the problem
        \begin{gather*}
            u''(x) + u'(x) = f(x)\\
            u'(0)=u(0)=\frac{1}{2}[u'(l)+u(l)], 
        \end{gather*}
        with $f(x)$ a given function.

        (a) Is the solution unique? Explain.\\
     Solution: \\
        Suppose we have two solutions $u_1,u_2$, and let $v=u_2-u_1$, then:
        \begin{align*}
            v''(x) + v'(x) &=(u_2-u_1)'' + (u_2-u_1)' \\
                           &= u_2''+u_2' - (u_1''+u_1') \\
                           &= f(x) - f(x) \\
                           &=0
        \end{align*}
        and also:
        \begin{align*}
            v'(0) =u_2'(0)-u_1'(0) = u_2(0)
            -u_1(0)&=\frac{1}{2}[u_2'(l)+u_2(l)]-\frac{1}{2}[u_1'(l)+u_1(l)]\\
                  &=\frac{1}{2}[u_2'(l)-u_1'(l) + u_2(l)-u_1(l)]\\
                  &=\frac{1}{2}[v'(l) + v(l)].
        \end{align*}
        This shows that $v$ satisfies the original problem with $f(x)=0$.

        Now, the ODE
        \[
        u''(x) + u'(x) = 0\\
        \]
        has the solution $A+Be^{-x}$. Using the initial conditions we get:
        \[
        u(x)=-2B+Be^{-x}
        \]
        This tells us that the solution is not unique because if we start with
        a solution we can add $-2B + Be^{-x}$ to it and get a different solution.
    
       (b) Does a solution necessarily exist, or is there a condition that $f(x)$ must satisfy for existence? Explain.\\
      Solution:\\
      From the beginning we can see that $f$ is the derivative of a function,
      namely the derivative of $u'+u$. This imposes some restrictions of $f$,
      for example $f$ cannot have jump discontinuities. So $f$ definitely can't be any function.\\
      Another condition for $f$ comes from the following: let $w=u'+u$, then
      $w$ must satisfy:
      \begin{equation*}
       \begin{cases}
           w'(x)=f(x),
           \\
           w(0)=w(l).
       \end{cases}
      \end{equation*}
      Which implies: $w(x)=\int_0^x f(s)ds +C$, and using the fact that
      $w(0)=w(l)$, we get:
      \[\int_0^0 f(s)ds+C=\int_0^l f(s)ds+C\]
Therefore, we obtain that a necessary condition for $f$ is $\int_{0}^{l}f(s)ds=0$.

        \item Exercise 3 \smallskip \\
        Solve the boundary problem $u'' = 0$ for $0 < x < 1$ with $u'\left(0\right) + ku\left(0\right) = 0$ and $u'\left(1\right) \pm ku\left(1\right) = 0$.  Do the $+$ and $-$ cases separately.  What is special about the case $k=2$? \\
        Solution: \\
      First, we consider the $+$ case. The equation is 
      \begin{equation*}
        \begin{cases}
            u'' = 0,
            \\
            u'\left(0\right) + ku\left(0\right) = 0,
            \\
            u'\left(1\right) + ku\left(1\right) = 0.
        \end{cases}
      \end{equation*}
    The general solution of $u(x)$ is $u(x)=ax+b$. From boundary conditions,
    \begin{equation*}
        \begin{cases}
            u'(0)+ku(0)=a+kb=0,
            \\
            u'(1)+ku(1)=a+k(a+b)=(1+k)a+kb=0.
        \end{cases}
    \end{equation*}
    Thus 
    $$
    u(x)=\begin{cases}
        b & \text{ if } k = 0, \\
        0 & \text{ if } k \ne 0.
      \end{cases}
   $$
   Then, consider the $-$ case. The equation is 
   \begin{equation*}
    \begin{cases}
        u'' = 0,
        \\
        u'\left(0\right) + ku\left(0\right) = 0,
        \\
        u'\left(1\right) - ku\left(1\right) = 0.
    \end{cases}
  \end{equation*}
  The general solution of $u(x)$ is still $u(x)=ax+b$. From boundary conditions,
    \begin{equation*}
        \begin{cases}
            u'(0)+ku(0)=a+kb=0,
            \\
            u'(1)-ku(1)=a-k(a+b)=(1-k)a-kb=0.
        \end{cases}
    \end{equation*}
    Thus $$
    u(x)=\begin{cases}
        b & \text{ if } k = 0, \\
        -2bx+b & \text{ if } k = 2, \\
        0 & \text{ if } k \ne 0 \text{ and } k \ne 2. 
      \end{cases}
   $$
        
For the special case $k=2$, in $+$ case, 
\begin{equation*}
    \begin{cases}
        u(x)=0,
        \\
        u'\left(0\right) + ku\left(0\right) = a+2b = 0,
        \\
        u'\left(1\right) + ku\left(1\right) = 3a+2b = 0.
    \end{cases}
\end{equation*}
There are two boundary conditions, the solution is unique, equal to 0.

For the special case $k=2$, in $-$ case,
\begin{equation*}
    \begin{cases}
        u(x)=-2bx+b,
        \\
        u'\left(0\right) + ku\left(0\right) = a+2b = 0,
        \\
        u'\left(1\right) + ku\left(1\right) = -a-2b = 0.
    \end{cases}
\end{equation*}
There's actually only one boundary condition, thus, the solution isn't unique, $u(x)=-2bx+b$.
    \end{enumerate}

    \pagebreak
    
    \item Strauss Section 1.6 \smallskip
    \begin{enumerate}
        \item Exercise 1 \smallskip \\
        What is the type of each of the following equations?
        \begin{enumerate}
            \item $u_{xx} - u_{xy} + 2u_y+u_{yy}-3u_{yx} + 4u = 0$. \smallskip \\
        Solution:\\
        Simplifying the equation: $u_{xx} - 4u_{xy} +u_{yy}+ 2u_y + 4u = 0.$
        
        From the general PDE form: $a_{11}u_{xx}+2a_{12}u_{xy}+a_{22}u_{yy}+a_{1}u_{x}+a_{2}u_{y}+a_{0}u=0.$
        
        Since $a_{11}=1,a_{12}=-2,a_{22}=1$, thus, $a_{12}^2=4, a_{11}a_{22}=1$, $a_{12}^2>a_{11}a_{22}$, hence this equation is Hyperbolic.
            
            \item $9u_{xx} + 6u_{xy} + u_{yy} + u_x = 0$. \smallskip \\
            Since $a_{11}=9,a_{12}=3,a_{22}=1$, thus, $a_{12}^2=9, a_{11}a_{22}=9$, $a_{12}^2=a_{11}a_{22}$, hence this equation is Parabolic.
        \end{enumerate}
        \item Exercise 6 \smallskip \\
        Consider the equation $3u_y + u_{xy} =0$.
        \begin{enumerate}
            \item What is its type? \smallskip \\
        Solution:\\
        Since $a_{11}=0,a_{12}=\frac{1}{2},a_{22}=0$, $a_{12}>a_{11}a_{22}$, this is Hyperbolic case.
            
            \item Find the general solution. (\emph{Hint:} Substitute $v = u_y$.) \smallskip \\
            Solution:\\
            Substitute $v = u_y$, the equation is $2v+v_{x}=0$. 

            By separating variables, we obtain $\frac{dv}{v}=-3dx$, and integrating both sides,
            we obtain:
            \[v(x,y)=e^{-3x}f(y).\]
            Then, \[u(x,y)=\int u_{y}dy= \int v(x,y) dy= F(y)e^{-3x}+g(x),\]  where $F'(y)=f(y)$ and $g(x)$ are arbitrary but sufficiently nice functions.
            
            \item With the auxiliary conditions $u\left(x,0\right) = e^{-3x}$ and $u_y\left(x,0\right)$, does a solution exist? Is it unique? \smallskip \\
            Solution:\\
            The PDE equation is 
            \begin{equation*}
                \begin{cases}
                    u(x,y)=F(y)e^{-3x}+g(x),
                    \\
                    u(x,0)=e^{-3x},
                    \\
                    u_{y}(x,0)=0
                \end{cases}
            \end{equation*}
            Then, we plug in the initial conditions to $u(x,y)=F(y)e^{-3x}+g(x)$, we get
            \begin{equation*}
                \begin{cases}
                    u(x,0)=F(0)e^{-3x}+g(x)=e^{-3x},
                    \\
                    u_{y}(x,0)=(f(y)e^{-3x})((x,0))=f(0)e^{-3x}=0.
                \end{cases}
            \end{equation*}
            These two equations imply:
            \begin{equation*}
                \begin{cases}
                    g(x)=e^{-3x}-F(0)e^{-3x}.
                    \\
                    f(0)=0,
                \end{cases}
            \end{equation*}
            Therefore, the solution is 
           \[u(x,y)=F(y)e^{-3x}+e^{-3x}-F(0)e^{-3x}=[F(y)-F(0)]e^{-3x}, F'(0)=0.\]
           Hence, the solution exist, as long as it satisfies the former
           equation, and for the function $F(y)$, $F'(0)=0$.
           
           Thus, the solution is not unique. 
           
           For example, $F(y)=ay^2$, $\forall a $ is a constant, there are infinite solutions $u(x,y)$ satisfying the equation.

            
        \end{enumerate}
    \end{enumerate}

    \pagebreak
    
    \item Strauss Section 2.1 \smallskip
    \begin{enumerate}
        \item Exercise 1 \smallskip \\
        Solve $u_{tt} = c^2u_{xx}$, $u\left(x,0\right) = e^x$, $u_t\left(x,0\right) = \sin{x}$. \smallskip \\
        Solution:\\
        Since $\phi(x)=u\left(x,0\right) = e^x$,$\psi(x)=u_t\left(x,0\right) = \sin{x}.$

        From the general formula for the wave equation with initial conditions,
        we know that
        \begin{align*}
            u(x,t)&=\frac{1}{2}[\phi(x+ct)+\phi(x-ct)]+\frac{1}{2c}\int_{x-ct}^{x+ct}\psi(s)ds\\
                  &=\frac{1}{2}[e^{x+ct}+e^{x-ct}]+\frac{1}{2c}\int_{x-ct}^{x+ct}\text{sin}(s)ds\\
                  &=\frac{1}{2}[e^{x+ct}+e^{x-ct}]+\frac{1}{2c}\text{cos}(x-ct)-\frac{1}{2c}\text{cos}(x+ct).
        \end{align*}
        \item Exercise 8 \smallskip \\
        A \emph{spherical wave} is a solution of the three-dimensional wave equation of the form $u\left(r,t\right)$ where $r$ is the distance to the origin (The spherical coordinate). The wave equation takes the form
        $$u_{tt} = c^2\left(u_{rr} + \frac{2}{r}u_r\right) \text{    ("spherical wave equation").}$$
        \begin{enumerate}
            \item Change variables $v= ru$ to get the equation for $v$:  $v_{tt} = c^2v_{rr}$. \smallskip \\
            Solution:\\
            Let $v=ru$, then $u=\frac{v}{r}$, thus, 
            \begin{equation}\label{v-equ}
                \begin{cases}
                    v_{r}=u+ru_{r},
                    \\
                    v_{rr}=2u_{r}+ru_{rr}.
                    \\
                    v_{tt}=ru_{tt},
                    \\
                    v_{t}=ru_{t},
                \end{cases}
            \end{equation}
            Plug (\ref{v-equ}) into equation $u_{tt} = c^2\left(u_{rr} + \frac{2}{r}u_r\right)$, i.e.
            \[ \frac{v_{tt}}{r}=c^2\left(\frac{v_{rr}-2u_r}{r}+\frac{2}{r}u_r\right)=c^2\frac{v_{rr}}{r}.\]
            Therefore, $v_{tt}=c^2v_{rr}$.
            \item Solve for $v$ using (3) and thereby solve the spherical wave equation. \smallskip \\
            Solution:\\
            From the general solution of wave equation, 
            \[ru(x,t)=v(x,t)=f(r-ct)+g(r+ct). \]
            Thus, $u(x,t)= \frac{1}{r}f(r-ct)+\frac{1}{r}g(r+ct). $
            Differentiating $u(x,t)$ about $t$,
            \begin{equation*}
                \begin{cases}
                    u_{t}=-\frac{c}{r}f'(r-ct)+\frac{c}{r}g'(r+ct),
                    \\
                    u_{tt}=\frac{c^2}{r}f''(r-ct)+\frac{c^2}{r}g''(r+ct),  
                \end{cases}
            \end{equation*}
            Differentiating $u(x,t)$ with respect to $r$,
            \[ u_{r}=-\frac{1}{r^2}f(r-ct)+\frac{1}{r}f'(r-ct)-\frac{1}{r^2}g(r+ct)+\frac{1}{r}g'(r+ct).\]
        Differentiating $u(x,t)$ with respect to $r$ again,
        \begin{align*}
            u_{rr}&=\frac{2}{r^3}f(r-ct)-\frac{1}{r^2}f'(r-ct)-\frac{1}{r^2}f'(r-ct) +\frac{1}{r}f''(r-ct) \\
               &+\frac{2}{r^3}g(r+ct)-\frac{1}{r^2}g'(r+ct)-\frac{1}{r^2}g'(r+ct) +\frac{1}{r}g''(r+ct)\\
               &=\frac{2}{r^3}f(r-ct)-\frac{2}{r^2}f'(r-ct)+\frac{1}{r}f''(r-ct) \\
               &+\frac{2}{r^3}g(r+ct)-\frac{2}{r^2}g'(r+ct)+\frac{1}{r}g''(r+ct).
        \end{align*}
         Thus, $u_{tt} = c^2\left(u_{rr} + \frac{2}{r}u_r\right)$, i.e. $u(x,t)$ is a solution of spherical wave equation.
           
            \item Use (8) to solve it with initial conditions $u\left(r,0\right) = \phi\left(r\right)$, $u_t\left(r,0\right) = \psi\left(r\right)$, taking both $\phi\left(r\right)$ and $\psi\left(r\right)$ to be even functions of $r$. \smallskip \\
            Solution:\\
            Since $v(r,t)$ is the solution of classical wave equation we will use (8) to help us solve it.
            From the initial condition of $u(r,t)$, we will obtain the initial condition of $v(r,t)$
            \begin{equation*}
                \begin{cases}
                    v(r,0)=ru(r,0)=r\phi(r),
                    \\
                    v_{t}(r,0)=ru_{t}(r,0)=r\psi(r).
                \end{cases}
            \end{equation*}
            And from (8), we know:
       \[v(x,t)=\frac{1}{2}[(r+ct)\phi(r+ct)+(r-ct)\phi(r-ct)]+\frac{1}{2c}\int_{r-ct}^{r+ct}s\psi(s)ds,\] therefore, the form of $u(r,t)$ is 
          \[u(r,t)=\frac{v(r,t)}{r}=\frac{1}{2r}[(r+ct)\phi(r+ct)+(r-ct)\phi(r-ct)]+\frac{1}{2cr}\int_{r-ct}^{r+ct}s\psi(s)ds\]
          This is the solution of spherical wave equation.
        \end{enumerate}
        
        \item Exercise 9 \smallskip \\
        Solve $u_{xx} - 3 u_{xt} - 4u_{tt} = 0$, $u\left(x,0\right) = x^2$, $u_t\left(x,0\right)$ = $e^x$. (\emph{Hint:} Factor the operator as we did for the wave equation.) \smallskip \\
        Solution:\\
        Using factor the operation to the wave equation: 
        \[u_{xx} - 3 u_{xt} - 4u_{tt}=(\partial x -4\partial t)(\partial x + \partial t) u=0.\]

        Then the second order wave equation will be transfered as two one order equations.
        \begin{equation*}
            \begin{cases}
                (\partial x + \partial t) u=v,
                \\
                (\partial x -4\partial t)v=0.
            \end{cases}
        \end{equation*}
        By using characteristic, $v(x,t)=f(x+\frac{1}{4}t)$, and $u(x,t)=f(x+\frac{1}{4}t)+g(x-t).$ 
        
        From the initial condition, 
        \begin{equation*}
            \begin{cases}
                u(x,0)=f(x)+g(x)=x^2,
                \\
                u_{t}(x,0)=\frac{1}{4}f_{t}(x)-g_{t}(x)=e^x.  
            \end{cases}
        \end{equation*}
        Intergrating $ u_{t}(x,0)=\frac{1}{4}f_{t}(x)-g_{t}(x)$ about $t$, then we get

        \[u(x,0)=\int u_{t}(x,0) dt =\int (\frac{1}{4}f_{t}(x)-g_{t}(x))dt=\frac{1}{4}f(x)-g(x)=e^x.\]
        Combinating equations:
        \begin{equation*}
            \begin{cases}
                u(x,0)=f(x)+g(x)=x^2,
                \\
                u(x,0)=\frac{1}{4}f(x)-g(x)=e^x.
            \end{cases}
        \end{equation*}
        We solve that 
        \begin{equation*}
            \begin{cases}
                f(x)=\frac{4}{5}(x^2+e^x+c),
                \\
                g(x)=\frac{1}{5}(x^2-4e^x-4c).
            \end{cases}
        \end{equation*}
        Therefore,
        \begin{align*}
            u(x,t)&=f(x+\frac{1}{4}t)+g(x-t)\\
            &=\frac{4}{5}[(x+\frac{1}{4}t)^2+e^{(x+\frac{1}{4}t)}+c] + \frac{1}{5}[(x-t)^2-4e^{(x-t)}-4c]\\
            &=\frac{4}{5}(x+\frac{1}{4}t)^2+\frac{4}{5}e^{(x+\frac{1}{4}t)}+\frac{1}{5}(x-t)^2- \frac{4}{5}e^{(x-t)}.
        \end{align*}
        Hence, $u(x,t)=\frac{4}{5}(x+\frac{1}{4}t)^2+\frac{4}{5}e^{(x+\frac{1}{4}t)}+\frac{1}{5}(x-t)^2- \frac{4}{5}e^{(x-t)}$ is the solution of this equation.
         \end{enumerate}

   \pagebreak
    
    \item Strauss Section 2.2 \smallskip
    \begin{enumerate}
        \item Exercise 1 \smallskip \\
        Use the energy conservation of the wave equation to prove that the only solution with $\phi \equiv 0$ and $\psi \equiv 0$ is $u \equiv 0$. (\emph{Hint:} Use the first vanishing theorem in Section A.1.) \smallskip \\
        Solution:\\
         First, we should show that $u\equiv0$ is a solution of the wave equation. Actually, it is trivial. 
        
        Since when $u=0$, thus $u_{tt}=0=u{xx}$, therefore, $u_{tt}=c^2u_{xx}$.
        
        Then, we should show $u=0$ is only solution with $\phi \equiv 0$ and $\psi \equiv 0$.
        
        Assume there exists another solution $v(x,t)\ne 0$ also satisfying wave equation, i.e. $v_{tt}=c^2v_{xx}.$

        Without loss of generalism, assume $v(x,t)> 0$, then by using energy equation
        \[ E(x,t)=\frac{1}{2}\int_{R} \left(v_{t}^{2}(x,t)+v_{x}^{2}(x,t)\right)dx\]

        Since the wave equation is energy conservation, i.e. $\frac{dE}{dt}=0.$ Therefore, $E = constant.$
        
        \[E(x,0)= \frac{1}{2}\int_{R}\left(v_{t}^{2}(x,0)+v_{x}^{2}(x,0)\right)dx=\frac{1}{2}\int_{R}\left(\psi^{2}+\phi_{x}^{2}\right)dx=\frac{1}{2}\int_{R}(0+0)dx =0.\]

        Thus $E(x,t)=E(x,0)=0.$

        And \[ 0=E(x,t)=\frac{1}{2}\int_{R} \left(v_{t}^{2}(x,t)+v_{x}^{2}(x,t)\right)dx,\] where $ v_{t}^{2}(x,t)+v_{x}^{2} (x,t)>0.$ 

        From Vanishing Theorem: $v_{t}^{2}(x,t)+v_{x}^{2}(x,t)=0 \implies v_{t}=0, v_{x}=0.$

        Hence, $ \nabla v(x,t)=(v_t(x,t),v_x(x,t))=(0,0),$ which means $v(x,t)=constant.$

        From initial condition, $v(x,0)= \phi =0$, thus, $v(x,t)=0, \forall x\in \mathbb{R}, t\ge 0.$

        Therefore, $u(x,t)=v(x,t)$, $u(x,t)\equiv 0$ is the only solution of wave equation with $\phi \equiv 0$ and $\psi \equiv 0$.
        
        %Let $f(x)$ be a continuous function in a finite closed interval [a,b]. Assume that $f(x)\ne 0$ in the interval and that $\int_{a}^{b}f(x)dx=0$. 
        %Then $f(x)$ is udentically zero.

        
        \item Exercise 2 \smallskip 

        For a solution $u\left(x,t\right)$ of the wave equation with $\rho = T = c = 1$, the energy density is defined as $e = \frac{1}{2}\left(u_t^2 + u_x^2\right)$ and the momentum density as $p =u_tu_x$.\smallskip 
        \begin{enumerate}
            \item Show that $\frac{\partial e}{\partial t} = \frac{\partial p}{\partial x}$ and $\frac{\partial p}{\partial t} = \frac{\partial e}{\partial x}$. \smallskip \\
            Solution: \\
            Since $e=\frac{1}{2}\left(u_{t}^{2}+u_{x}^{2}\right)$, $p=u_{t} u_{x} $.
            \begin{equation*}
                \begin{cases}
                    \frac{\partial e}{\partial t}=u_{t} u_{tt}+u_{xt} u_{x},
                    \\
                    \frac{\partial p}{\partial x}=u_{xt} u_{x}+u_{t} u_{xx}.
                \end{cases}
            \end{equation*}
            Thus, \[\frac{\partial e}{\partial t}=u_{t} u_{t t}+u_{x t} u_{x}=u_{t} u_{x x}+u_{x t} u_{x}=\frac{\partial p}{\partial x} .\]
            Also
            \begin{equation*}
                \begin{cases}
                    \frac{\partial p}{\partial t}=u_{tt} u_{x}+u_{t} u_{xt},
                    \\
                    \frac{\partial e}{\partial x}=u_{t} u_{tx}+u_{x} u_{xx}.
                \end{cases}
            \end{equation*}
            Hence, \[\frac{\partial p}{\partial t}=u_{tt} u_{x}+u_{t} u_{xt}=u_{t} u_{tx}+u_{x} u_{xx}=\frac{\partial e}{\partial x} .\]
            


            \item Show that both $e\left(x,t\right)$ and $p\left(x,t\right)$ also satisfy the wave equation.    
           
            Solution:\\
             First, we consider $e(x,t).$
            \[e_{tt}  =\frac{\partial}{\partial t}\left(u_{t} u_{tt}+u_{x} u_{xt}\right)=u_{tt} u_{tt}+u_{t} u_{ttt}+u_{xtt} u_{x}+u_{xt} u_{xt},\]          
            \[ e_{xx}  =\frac{\partial}{\partial x}\left(u_{t} u_{tx}+u_{x} u_{xx}\right) =u_{tx} u_{tx}+u_{t} u_{txx}+u_{xx} u_{xx}+u_{x} u_{xxx}. \]
            
            Since $u_{xx}=u_{tt}$, then 
            \[ e_{tt}=u_{tt} u_{tt}+u_{t} u_{ttt}+u_{xtt} u_{x}+u_{xt} u_{xt}=u_{tx} u_{tx}+u_{t} u_{txx}+u_{xx} u_{xx}+u_{x} u_{xxx}=e_{xx}. \]
            
            Therefore, $e(x,t)$ satisfies the wave equation.
            

            Then, we check $p(x,t).$
            \[p_{tt}  =\frac{\partial}{\partial t}\left(u_{tt} u_{x}+u_{t} u_{xt}\right)=u_{ttt} u_{x}+u_{tt} u_{xt}+u_{tt} u_{xt}+u_{t} u_{xtt},\]          
            \[ p_{xx}  =\frac{\partial}{\partial x}\left(u_{xt} u_{x}+u_{t} u_{xx}\right) =u_{xxt} u_{x}+u_{xt} u_{xx}+u_{tx} u_{xx}+u_{t} u_{xxx}. \]
            since $u_{xx}=u_{tt}$, then 
            \[ p_{tt}=u_{ttt} u_{x}+u_{tt} u_{xt}+u_{tt} u_{xt}+u_{t} u_{xtt}=u_{xxt} u_{x}+u_{xt} u_{xx}+u_{tx} u_{xx}+u_{t} u_{xxx}=p_{xx}. \]
            
            Therefore, $p(x,t)$ satisfies the wave equation.
        \end{enumerate}
    \end{enumerate}
    
    \pagebreak

    \item Strauss Section 2.3 \smallskip
    \begin{enumerate}
        \item Exercise 1 \smallskip \\
        Consider the solution $1 - x^2 -2kt$ of the diffusion equation.  Find the locations of its maximum and its minimum in the closed rectangle $\{0 \leq x \leq 1, 0 \leq t \leq T\}$. \smallskip \\
          Solution:\\
          By the maximum principle, the maximum and minimum values are attained
          at the boundary.
          We start finding for the maximum.

          First we set $t=0$. And we get $1-x^2$ which has a maximum of 1, then
          if we set $x=0$ we get $1-2kt$ which has 1 as the maximum, then
          if we set $x=1$ we get $-2kt$ which has 0 as the maximum.

          In conclusion: the maximum is 1 and it is attained at $x=0,t=0$.
          
          Now we find the minimum in the same way.

          First we set $t=0$. And we get $1-x^2$ which has a minimum of 0, then
          if we set $x=0$ we get $1-2kt$ which has $1-2kT$ as the minimum, then
          if we set $x=1$ we get $-2kt$ which has $-2kT$ as the minimum.

          In conclusion: the minimum is $-2kT$ and it is attained at $x=1,t=T$.
    \end{enumerate}
\end{enumerate}

\end{document}
